

Directions: Determine if the following rational functions have a horizontal asymptote, a slant asymptote, or neither.

$$1. f(x) = \frac{2x^2 - 3x + 5}{5x^2 - 6}$$

Horizontal $y = \frac{2}{5}$ because the quotient of the leading terms $\frac{2x^2}{5x^2} = \frac{2}{5}$.

$$2. r(x) = \frac{2x^2 - 4x + 7}{6 - 5x}$$

Slant because the quotient of the leading terms $\frac{2x^2}{-5x} = -\frac{2}{5}x$ is linear.

$$3. h(x) = \frac{x^3 - 2x + 5}{3x - 4}$$

Neither because the quotient of the leading terms $\frac{x^3}{3x} = \frac{1}{3}x^2$ is not linear.

$$4. k(x) = \frac{x^4 - 3x^2 + x - 9}{2x^3 - x + 7}$$

Slant because the quotient of the leading terms $\frac{x^4}{2x^3} = \frac{1}{2}x$ is linear.

$$5. g(x) = \frac{x^2 - x - 1}{x^3 + x^2 - 2}$$

Horizontal $y = 0$ because the quotient of the leading terms $\frac{x^2}{x^3} = \frac{1}{x}$ is not linear. It has a constant numerator and nonconstant denominator.

$$6. y = \frac{(x-2)^2(3x^2+2)}{x(x+1)(x-5)}$$

Slant because the quotient of the leading terms $\frac{3x^4}{x^3} = 3x$ is linear.

Directions: For each rational function below, use long division to find the equation of the slant asymptote.

$$7. f(x) = \frac{x^2 - 6x + 7}{x - 1}$$

Slant asymptote: $y = x - 5$

$$\begin{array}{r} x-5 \\ x-1 \overline{) x^2 - 6x + 7} \\ \underline{x^2 - x} \\ -5x + 7 \\ \underline{-5x + 5} \\ 2 \end{array}$$

$$8. g(x) = \frac{2x^2 - x + 4}{x + 3}$$

Slant asymptote: $y = 2x - 7$

$$\begin{array}{r} 2x-7 \\ x+3 \overline{) 2x^2 - x + 4} \\ \underline{2x^2 + 6x} \\ -7x + 4 \\ \underline{-7x - 21} \\ 25 \end{array}$$

$$9. h(x) = \frac{x^3 - 4x^2 + 3x - 1}{x^2 - 2x + 5}$$

Slant asymptote: $y = x - 2$

$$\begin{array}{r} x-2 \\ x^2-2x+5 \overline{) x^3 - 4x^2 + 3x - 1} \\ \underline{x^3 - 2x^2 + 5x} \\ -2x^2 - 2x - 1 \\ \underline{-2x^2 + 4x - 10} \\ -6x + 9 \end{array}$$

$$10. k(x) = \frac{2x^3 - x^2 + 1}{x^2 + x + 1}$$

Slant asymptote: $y = 2x - 3$

$$\begin{array}{r} 2x-3 \\ x^2+x+1 \overline{) 2x^3 - x^2 + 0x + 1} \\ \underline{2x^3 + 2x^2 + 2x} \\ -3x^2 - 2x + 1 \\ \underline{-3x^2 - 3x - 3} \\ x + 4 \end{array}$$